Amend definitions of labeled things.
The main reason for this change is to make the proj_node_state_to_proj_n
provable, while still supporting creating/destroying nodes and channels
that are labeled secret.

The main change is that for objects that have labels:
- labels are now decoupled from the rest of the object
- the objects are replaced by options, and empty versions are really
none. This is done with the definition "labeled" in RuntimeModel.v

To give confidence that this change makes forward progress, note that
- secret labeled objects holding a None are indistinguishable from real
ones, so this does not undo the change in
[#1603](https://github.com/project-oak/oak/pull/1603)
- If a nid/handle points to a real object in a projected state, it does
also guarantee the same is true in the non-projected state, making the
troublesome theorem provable.

As a side-effect the definitions of several theorems in NIUtilTheorems
get better reuse, and the low projections are also probably more
trustworthy since they are more clearly distinguished from real objects.

experimental/ni_coq/vfiles/LowEquivalences.v
@@ -10,6 +10,9 @@ From OakIFC Require Import
     RuntimeModel
     EvAugSemantics.
 
+From RecordUpdate Require Import RecordSet.
+Import RecordSetNotations.
+
 (* Ensembles don't have implicit type params and this line fixes that *)
 Arguments Ensembles.Empty_set{U}.
 
@@ -29,52 +32,33 @@ are related even if their contents differ.
 
 
 (*============================================================================
-* Empty Things
-*===========================================================================*)
-Definition empty_chan (l:level): channel := {|
-    clbl := l;
-    ms := [];
-|}.
-
-Definition empty_node (l: level): node := {|
-    nlbl := l;
-    read_handles := Empty_set;
-    write_handles := Empty_set;
-    ncall := Internal; 
-|}.
-
-Definition empty_event (l: level): event_l := {|
-    elbl := l;
-    e := NilEv;
-|}.
-    
-
-(*============================================================================
 * Low Projections
 *===========================================================================*)
 
-Definition low_proj (A: Type): Type := level -> A -> A.
+Definition low_proj_t {A: Type}: Type := level -> A -> A.
+Definition low_proj {A: Type} ell ( labeled_thing: @labeled A) := 
+    match labeled_thing with
+        | Labeled _ o ell' => if( ell' <<? ell ) 
+            then labeled_thing
+            else Labeled A None ell'
+    end.
 
-Definition chan_low_proj (ell: level)(c: channel): channel :=
-    if(c.(clbl) <<? ell) then c else (empty_chan c.(clbl)).
+Definition node_low_proj := @low_proj node.
+Definition chan_low_proj := @low_proj channel.
+Definition event_low_proj := @low_proj event.
 
-Definition node_low_proj (ell: level)(n: node): node :=
-    if(n.(nlbl) <<? ell) then n else (empty_node n.(nlbl)).
-
-Definition event_low_proj (ell: level)(e: event_l): event_l :=
-    if(e.(elbl) <<? ell) then e else (empty_event e.(elbl)).
 
 Definition node_state_low_proj (ell: level)(ns: node_state): node_state :=
-    fun id => match (ns id) with
-        | None => Some (empty_node ell)
-        | Some n => Some (node_low_proj ell n)
-    end.
+    fun id => 
+        if (ns id).(lbl) <<? ell 
+            then (ns id)
+            else low_proj ell (ns id).
 
 Definition chan_state_low_proj (ell: level)(cs: chan_state): chan_state :=
-    fun h => match (cs h) with
-        | None => Some (empty_chan ell)
-        | Some c => Some (chan_low_proj ell c)
-    end.
+    fun h => 
+        if (cs h).(lbl) <<? ell
+            then (cs h)
+            else low_proj ell (cs h).
 
 Definition state_low_proj (ell: level)(s: state): state := {|
     nodes := node_state_low_proj ell s.(nodes);
@@ -85,15 +69,19 @@ Definition state_low_proj (ell: level)(s: state): state := {|
 * Low Equivalences
 *===========================================================================*)
 
-Definition low_eq {A: Type} (p: (low_proj A)):=
-    fun ell a1 a2 => (p ell a1) = (p ell a2).
+Definition low_eq_t {A: Type}: Type := level -> A -> A -> Prop.
+Definition low_eq {A: Type} ell (x: @labeled A) (y: @labeled A) :=
+    (low_proj ell x) = (low_proj ell y).
 
-Definition chan_low_eq := low_eq chan_low_proj.
-Definition node_low_eq := low_eq node_low_proj.
-Definition event_low_eq := low_eq event_low_proj.
-Definition node_state_low_eq := low_eq node_state_low_proj.
-Definition chan_state_low_eq := low_eq chan_state_low_proj.
-Definition state_low_eq := low_eq state_low_proj.
+Definition chan_low_eq := @low_eq channel.
+Definition node_low_eq := @low_eq node.
+Definition event_low_eq := @low_eq event.
+Definition node_state_low_eq := fun ell ns1 ns2 => 
+    (node_state_low_proj ell ns1) = (node_state_low_proj ell ns2).
+Definition chan_state_low_eq := fun ell cs1 cs2 =>
+    (chan_state_low_proj ell cs1) = (chan_state_low_proj ell cs2).
+Definition state_low_eq := fun ell s1 s2 =>
+    (state_low_proj ell s1) = (state_low_proj ell s2).
 
 (*============================================================================
 * Trace Low Equivalences
