experimental/ni_coq/vfiles/Events.v
@@ -8,25 +8,10 @@ Import ListNotations.
 (* This file contains  *)
 
 Inductive event: Type :=
-    | NilEv: event
     | InEv (m: message): event
     | OutEv (m: message): event
-    | NCreateEv (n: node): event.
+    | NCreateEv: event.
 (* note that messages include the bytes and handles sent via channels *)
 (* eventually, downgrades will also be represented by events *)
 
-Record event_l := EvL {
-    e :event;
-    elbl: level;
-}.
-
-(*
-Inductive ev_low_eq: level -> event_l -> event_l -> Prop :=
-    | EvEq ell el1 el2: 
-            el1 = el2 ->
-            ev_low_eq ell el1 el2
-    | EvNoFlow ell el1 el2:
-        ~((lvl el2) <<L ell) ->
-        ~((lvl el1) <<L ell) ->
-        ev_low_eq ell el1 el2.
-*)
+Definition event_l := @labeled event.
